Propagated entry_point stackframe to all languages.
There are now various holes in almost every transl_entry_points proof.

backend/Cminor.v
@@ -608,15 +608,20 @@ Inductive initial_state (p: program): state -> Prop :=
       funsig f = signature_main ->
       initial_state p (Callstate f nil Kstop m0).
 
+Require Import Conventions.
+
 Inductive entry_point (p: program): mem -> state -> val -> list val -> Prop :=
-  | entry_point_intro: forall b f m0 args,
+  | entry_point_intro: forall b f b0 f0 m0 m1 stk args,
       let ge := Genv.globalenv p in
       Mem.mem_wd m0 ->
       Mem.arg_well_formed args m0 ->
       globals_not_fresh ge m0 ->
       Genv.find_funct_ptr ge b = Some f ->
       Val.has_type_list args (sig_args (funsig f)) ->
-      entry_point p m0 (Callstate f args Kstop m0) (Vptr b Ptrofs.zero) args.
+      Genv.find_funct_ptr ge b0 = Some (Internal f0) ->
+      tailcall_possible (fn_sig f0) ->
+      Mem.alloc m0 0 0 = (m1, stk) ->
+      entry_point p m0 (Callstate f args (Kcall None f0 (Vptr stk Ptrofs.zero) (PTree.empty _) Kstop) m1) (Vptr b Ptrofs.zero) args.
 
 (** A final state is a [Returnstate] with an empty continuation. *)
 
@@ -1217,6 +1222,8 @@ Proof.
   traceEq.
 Qed.
 
+(* Because of the handler, entry_point isn't suitable for use as the initial state of the program,
+   but that's how Smallstep.initial_state is defined. *)
 Theorem bigstep_semantics_sound:
   bigstep_sound (bigstep_semantics prog) (semantics prog).
 Proof.
@@ -1224,7 +1231,8 @@ Proof.
     intros.
 -(* termination *)
   inv H. econstructor; econstructor.
-  split. econstructor; eauto.
+  admit.
+(*  split. econstructor; eauto.
   econstructor; eauto.
   + eapply Genv.initmem_inject; eauto.
   + constructor.
@@ -1232,18 +1240,19 @@ Proof.
     erewrite Genv.init_mem_genv_next; eauto; reflexivity.
   + rewrite H3; simpl; auto.
   + split. apply eval_funcall_steps. eauto. red; auto.
-  econstructor.
+  econstructor.*)
 -(* divergence *)
   inv H. econstructor.
   split. econstructor; eauto.
-         econstructor; eauto.
+  admit.
+(*         econstructor; eauto.
          eapply Genv.initmem_inject; eauto.
          constructor.
          unfold globals_not_fresh.
          erewrite Genv.init_mem_genv_next; eauto; reflexivity.
-         rewrite H3; simpl; auto.
+         rewrite H3; simpl; auto.*)
   eapply forever_plus_forever.
   eapply evalinf_funcall_forever; eauto.
-Qed.
+Admitted.
 
 End BIGSTEP_TO_TRANSITION.
