cfrontend/Clight.v
@@ -759,22 +759,30 @@ Inductive val_casted_list: list val -> typelist -> Prop :=
       val_casted v1 ty1 -> val_casted_list vl tyl ->
       val_casted_list (v1 :: vl) (Tcons  ty1 tyl).
 
+Require Import Conventions.
+
+Definition loc_arguments' l := if Archi.ptr64 then loc_arguments_64 l 0 0 0 else loc_arguments_32 l 0.
+
 (*NOTE: DOUBLE CHECK TARGS (it's not used right now)*)
 Inductive entry_point (ge:genv): mem -> state -> val -> list val -> Prop :=
 | initi_core:
-    forall f fb m args targs tres,
+    forall f fb b0 f0 m0 m1 stk args targs tres,
       Genv.find_funct_ptr ge fb = Some f ->
       type_of_fundef f = Tfunction targs tres cc_default ->
-      globals_not_fresh ge m ->
-      Mem.mem_wd m ->
-      Mem.arg_well_formed args m ->
+      globals_not_fresh ge m0 ->
+      Mem.mem_wd m0 ->
+      Mem.arg_well_formed args m0 ->
       val_casted_list args targs ->
       Val.has_type_list args (typlist_of_typelist targs) ->
       (*val_casted_list_func args targs 
                            && tys_nonvoid targs 
                            && vals_defined args
                            && zlt (4*(2*(Zlength args))) Int.max_unsigned = true ->*)
-      entry_point ge m (Callstate f args Kstop m) (Vptr fb (Ptrofs.of_ints Int.zero)) args.
+      Genv.find_funct_ptr ge b0 = Some (Internal f0) ->
+      (forall l, In l (regs_of_rpairs (loc_arguments' (map typ_of_type (map snd (fn_params f0))))) ->
+        match l with Locations.R _ => True | Locations.S _ _ _ => False end) ->
+      Mem.alloc m0 0 0 = (m1, stk) ->
+      entry_point ge m0 (Callstate f args (Kcall None f0 (PTree.empty _) (PTree.empty _) Kstop) m1) (Vptr fb Ptrofs.zero) args.
 
 (** A final state is a [Returnstate] with an empty continuation. *)
 Inductive final_state: state -> int -> Prop :=
