x86/Asmgenproof.v
@@ -882,31 +882,30 @@ Proof.
   auto.
 Qed.
 
-Lemma set_arg_PC:
-  forall rs l v,
-  set_arg rs l v PC = rs PC /\ set_arg rs l v RA = rs RA.
-Proof.
-  destruct l; auto; simpl; intros.
-  rewrite !Pregmap.gso; auto with asmgen.
-Qed.
-
-Lemma set_arguments_PC:
-  forall rs l v rs', set_arguments rs l v = Some rs' ->
+Lemma make_arg_PC:
+  forall rs rs' m m' l v, make_arg rs m l v = Some (rs', m') ->
   rs' PC = rs PC /\ rs' RA = rs RA.
 Proof.
-  intros until l; revert rs; induction l; simpl; intros.
-  - inv H; auto.
+  destruct l; auto; simpl; intros.
+  - inv H.
+    rewrite !Pregmap.gso; auto with asmgen.
+  - destruct (Mem.storev _ _ _ _); inv H; auto.
+Qed.
+
+Lemma make_arguments_PC:
+  forall rs rs' m m' l v, make_arguments rs m l v = Some (rs', m') ->
+  rs' PC = rs PC /\ rs' RA = rs RA.
+Proof.
+  intros until l; revert rs' m'; induction l; simpl; intros.
+  - destruct v; inv H; auto.
   - destruct v; try discriminate.
-    { inv H; auto. }
-    destruct (set_arguments _ _) eqn: Ha; try discriminate.
+    destruct (make_arguments _ _ _ _) as [[]|] eqn: Ha; try discriminate.
     apply IHl in Ha as [<- <-].
     destruct a.
-    + inv H; apply set_arg_PC.
-    + destruct v; inv H.
-      * destruct (set_arg_PC r rhi Vundef) as [<- <-].
-        apply set_arg_PC.
-      * destruct (set_arg_PC r rhi (Vint (Int64.hiword i))) as [<- <-].
-        apply set_arg_PC.
+    + eapply make_arg_PC; eauto.
+    + destruct (make_arg _ _ _ _) as [[]|] eqn: Ha; try discriminate.
+      eapply make_arg_PC in Ha as [<- <-].
+      eapply make_arg_PC; eauto.
 Qed.
 
 Lemma transf_entry_points:
@@ -915,22 +914,25 @@ Lemma transf_entry_points:
   exists s2 : Asm.state, Asm.entry_point tge m0 s2 f arg /\ match_states s1 s2.
 Proof.
   intros. inv H. subst ge0.
-  exploit functions_translated; eauto. intros (tf & A & B).
-  exploit set_arguments_match; eauto.
+  destruct (functions_translated b f0) as (tf & A & B); auto.
+  destruct (functions_translated b0 (Internal f1)) as (tf0 & A0 & B0); auto; simpl in B0.
+  destruct (transf_function f1) eqn: Hf1; inv B0.
+  exploit make_arguments_match; eauto.
   { instantiate (1 := (Pregmap.init Vundef)
         # PC <- (Vptr b Ptrofs.zero) 
-        # RA <- Vzero
-        # RSP <- Vnullptr).
+        # RA <- Vnullptr
+        # RSP <- (Vptr stk Ptrofs.zero)).
     constructor; auto; discriminate. }
   intros (rs' & ? & ?).
   econstructor; split.
   - econstructor; eauto.
     erewrite sig_preserved; eauto.
-  - eapply set_arguments_PC in H as [HPC HRA].
+  - eapply make_arguments_PC in H as [HPC HRA].
     econstructor; eauto.
-    + constructor.
+    + repeat econstructor; eauto; try discriminate.
+      admit. (* return address shouldn't be null *)
     + apply Mem.extends_refl.
-Qed.
+Admitted.
 
 Lemma transf_initial_states:
   forall st1, Mach.initial_state prog st1 ->
